verification/tests/TestOpenList.fst
@@ -3,14 +3,14 @@ open FStar.List.Tot
 open FStar.Char
 open FStar.String
 
-let rec f (fuel:int) (cs:list char) (acc:int) : Tot (int * (list char)) (decreases fuel) =
+let rec f (fuel:int) (cs:list char) (acc:int) : Tot (int & list char) (decreases fuel) =
   if fuel <= 0 then (acc, cs)
   else match cs with
   | _ :: rest -> f (fuel - 1) rest acc
   | [] -> (acc, cs)
 
-and g (fuel:int) (cs:list char) (acc:list char) : Tot (string * (list char)) (decreases fuel) =
+and g (fuel:int) (cs:list char) (acc:list char) : Tot (string & list char) (decreases fuel) =
   if fuel <= 0 then ("", cs)
   else match cs with
-  | _ :: rest -> g (fuel - 1) rest (c :: acc)
+  | _ :: rest -> g (fuel - 1) rest ('a' :: acc)
   | [] -> ("", [])
